\section{Relational probabilities}

The \emph{subset} relation, denoted by the predicate
\begin{equation}
    \subseteq \colon \PS{\Set{U}} \times \PS{\Set{U}} \mapsto 
    \{\True,\False\}\,,
\end{equation}
is \True if every element of the first set is in the second set and otherwise
\False.

\begin{theorem}
Given $\Set{X} \subseteq \Set{Y}$, $\ASet{X} \subseteq \ASet{Y}$ with probability
\begin{equation}
    \left(1 - \tprate_1(1 - \tprate_2)\right)^{\Card{\Set{X}}}
    \left(1 - \fprate_1(1 - \tprate_2)\right)^{\Card{\Set{Y}} - \Card{\Set{X}}}
    \left(1 - \fprate_1(1 - \fprate_2)\right)^{\Card{\Set{U}} - 
    \Card{\Set{Y}}}\,.
\end{equation}
\end{theorem}
\begin{proof}
Let
\begin{equation}
    \gamma = \Prob{\ASet{X} \subseteq \ASet{Y} \Given \Set{X} \subseteq 
    \Set{Y}}\,.
\end{equation}

Note that in the Boolean vector representation, $\Set{X}$ is a subset of 
$\Set{Y}$ if $x_j \implies y_j$, i.e., if $x_j$ then $y_j$, otherwise $y_j$ can 
be either true or false. An equivalent expression for $x_j \implies y_j$ is 
$\neg (x_j \land \neg y_j)$.

Switching to the Boolean vector representation, we may rewrite $\gamma$ as
\begin{equation}
    \gamma = \Prob{\bigcap_{j=1}^{u} \neg \left(\AVecComp{X}[j] \land \neg 
    \AVecComp{Y}[j]\right) \Given E}
\end{equation}
where $E$ is the set of Boolean vectors satisfying $x_k \implies y_k$ for     
$k=1,\ldots,u$.

By the axioms of the approximate set model, each of these events are 
independent, in which case the probability of the intersection of the events is 
equal to the product of the probabilities of the events,
\begin{align}
\gamma
    &= \prod_{j=1}^{u} \Prob{\neg\left(\AVecComp{X}[j] 
        \land \neg \AVecComp{Y}[j]\right) \Given E}\\
    &= \prod_{j=1}^{u} \left(1 - \Prob{\AVecComp{X}[j] 
        \land \neg \AVecComp{Y}[j] \Given E}\right)\,.
\end{align}
By the axioms of the approximate set model, $\AVecComp{Y}[j]$ is only dependent 
on $y_j$ and $\AVecComp{X}[j]$ is only dependent on $x_j$. Thus, we may rewrite 
$\gamma$ as
\begin{equation}
\gamma = \prod_{j=1}^{u}\left(
    1 - \Prob{\AVecComp{X}[j] \Given x_j}
    \Prob{\neg \AVecComp{Y}[j] \Given y_j}\right)\,,
\end{equation}
where $x_j$ and $y_j$ are Boolean values satisying $E$.

Since $\Set{X} \subseteq \Set{Y}$, an exhaustive, mutually exclusive set of 
sets is given by $\Set{X}$, $\SetDiff[\Set{Y}][\Set{X}]$, and 
$\SetComplement[\Set{Y}]$.

Let set $\Set{I}$ index the elements in $\Set{X}$, set $\Set{J}$ index 
the elements in $\SetDiff[\Set{Y}][\Set{X}]$, and set $\Set{K}$ index the 
elements in $\SetComplement[\Set{Y}]$.

The elements indexed by $\Set{I}$ are members of $\Set{X}$ and $\Set{Y}$, i.e.,
$x_i$ and $y_i$ are both true.

The elements indexed by $\Set{J}$ are members of $\Set{Y}$ but not $\Set{X}$,
i.e., $x_j$ is false and $y_j$ is true.

The elements indexed by $\Set{K}$ are members of neither, i.e., $x_j$ and $y_j$
are false.


\begin{equation}
\begin{split}
\gamma =
    &\prod_{i \in \Set{I}}
        \left(1-\Prob{\AVecComp{X}[i] \Given x_i}
        \Prob{\neg \AVecComp{Y}[i] \Given y_i}\right)
    \prod_{j \in \Set{J}}
        \left(1-\Prob{\AVecComp{X}[j] \Given \neg x_j}
        \Prob{\neg \AVecComp{Y}[j] \Given y_j}\right)\\
    &\qquad \prod_{k \in \Set{K}}
        \left(1-\Prob{\AVecComp{X}[k] \Given \neg x_k}
        \Prob{\neg \AVecComp{Y}[k] \Given \neg y_k}\right)\,.  
\end{split}    
\end{equation}



\begin{equation}
\gamma =
    \prod_{i \in \Set{I}}
        \left(1 - \tprate_1
        (1 - \tprate_2)\right)
    \prod_{j \in \Set{J}}
        \left(1 - \fprate_1
        (1 - \tprate_2)\right)
    \prod_{k \in \Set{K}}
        \left(1 - \fprate_1
        (1 - \fprate_2)\right)
\end{equation}



\begin{equation}
\gamma =
\prod_{i \in \Set{I}}
\left(1 - \tprate_1
(1 - \tprate_2)\right)
\prod_{j \in \Set{J}}
\left(1 - \fprate_1
(1 - \tprate_2)\right)
\prod_{k \in \Set{K}}
\left(1 - \fprate_1
(1 - \fprate_2)\right)
\end{equation}



By \cref{dummyrefs}, $\Prob{x \in \ASet{X} \Given x \in \Set{X}} = \tprate_1$, 
$\Prob{x \in \ASet{X} \Given x \notin \Set{X}} = \fprate_1$, $\Prob{x \in 
\ASet{Y} \Given x \in \Set{Y}} = \tprate_2$, and $\Prob{x \in \ASet{Y} \Given x 
\notin \Set{Y}} = \fprate_1$. Making these substitutions yields the result
\begin{equation}
\begin{split}
\gamma =
    &\prod_{x \in \Set{V}[1]}
    \left(1 -
        \tprate_1
        (1 - \tprate_2)
    \right)\\
    &\prod_{x \in \Set{V}[2]}
    \left(1 -
        \fprate_1
        (1 - \tprate_2)
    \right)\\
    &\prod_{x \in \Set{V}[3]}
    \left(1 -
        \fprate_1
        (1 - \fprate_2)
    \right)\,.  
\end{split}    
\end{equation}
Each of the above products is just repeated multiplication and thus may be 
replaced by powers,
\begin{equation}
\begin{split}
\gamma &=
    \left(1 - \tprate_1(1 - \tprate_2)\right)^{\Card{\Set{V}[1]}}\\
    &\qquad \left(1 - \fprate_1(1 - \tprate_2)\right)^{\Card{\Set{V}[2]}}
    \left(1 - \fprate_1(1 - \fprate_2)\right)^{\Card{\Set{V}[3]}}\,.  
\end{split}
\end{equation}
\end{proof}